

CHAPTER 2 : POLYNOMIALS

- **Question 1:** Write the degree of the polynomial $x^2 - 5x + 6$.
Question 2: Identify the coefficient of x in $3x^3 - 7x + 2$.
Question 3: Determine the remainder when $x^3 - 2x^2 + 4$ is divided by $x - 1$.
Question 4: Write a polynomial of degree 2.
Question 5: Is $x^2 + 1$ a linear polynomial?
- **Question 6:** Check whether $x - 2$ is a factor of $x^3 - 3x^2 + 4x - 8$.
Question 7: Find the remainder when $x^3 + x^2 - x + 2$ is divided by $x + 1$.
Question 8: If α and β are zeroes of $x^2 - 5x + 6$, find $\alpha + \beta$.
Question 9: Find the product of zeroes of $2x^2 - 3x + 1$.
Question 10: Find the sum of zeroes of $3x^2 + 7x - 6$.

Question 11: Verify that 1 and -2 are zeroes of $x^2 + x - 2$.

Question 12: If α and β are zeroes of $x^2 - 3x + 2$, form a quadratic polynomial whose zeroes are $\alpha + 1$ and $\beta + 1$.

Question 13: Find a quadratic polynomial whose sum of zeroes = 5 and product = 6.

Question 14: Find the zeroes of $2x^2 - 5x - 3$ and verify relationship with sum and product.

Question 15: If α and β are zeroes of $x^2 - x - 6$, find a polynomial whose zeroes are $1/\alpha$ and $1/\beta$.

Question 16: Verify that the zeroes of $x^2 - 5x + 6$ satisfy $\alpha^2 + \beta^2 = (\alpha + \beta)^2 - 2\alpha\beta$.

Question 17: Find a quadratic polynomial whose zeroes are 2 more than the zeroes of $x^2 - 3x + 2$.

Question 18: Find a cubic polynomial with zeroes 1, -2 , 3.

Question 19: If α and β are zeroes of $2x^2 - 5x + 3$, verify that $1/\alpha + 1/\beta = (\alpha + \beta)/(\alpha\beta)$.

Question 20: If α, β, γ are zeroes of $x^3 - 6x^2 + 11x - 6$, find $\alpha\beta + \beta\gamma + \gamma\alpha$.

Question 21: Check whether $x - 3$ is a factor of $x^3 - 4x^2 + x + 6$.

Question 22: Find the remainder when $x^3 + 2x^2 - 5x + 4$ is divided by $x - 2$.

Question 23: Find a quadratic polynomial whose zeroes are squares of zeroes of $x^2 - 3x + 2$.

Question 24: If α, β are zeroes of $x^2 - 2x - 3$, find a polynomial whose zeroes are $\alpha - 1$ and $\beta - 1$.

Question 25: Find the sum of cubes of zeroes of $x^2 - 5x + 6$.

Question 26: Find a quadratic polynomial whose zeroes are reciprocals of zeroes of $x^2 - x - 6$.

Question 27: If α, β, γ are zeroes of $x^3 - 3x^2 + 4x - 2$, find $\alpha^2 + \beta^2 + \gamma^2$.

Question 28: Verify that zeroes of $x^2 - 7x + 12$ satisfy $\alpha^2 - \beta^2 = (\alpha - \beta)(\alpha + \beta)$.

Question 29: Find the cubic polynomial whose zeroes are 1, -1 , 2.

Question 30: Find the remainder when $2x^3 + 3x^2 - x + 5$ is divided by $x + 1$.

HINTS/SOLUTION

Solution 1:

Polynomial: $x^2 - 5x + 6$

Degree of a polynomial = highest power of $x \rightarrow 2$

Answer: 2

Solution 2:

Polynomial: $3x^3 - 7x + 2$

Coefficient of x = number multiplying $x \rightarrow -7$

Answer: -7

Solution 3:

Polynomial: $x^3 - 2x^2 + 4$

Divide by $x - 1 \rightarrow$ Use Remainder Theorem

Remainder = $f(1) = (1)^3 - 2(1)^2 + 4 = 1 - 2 + 4 = 3$

Answer: 3

Solution 4:

Polynomial of degree 2 \rightarrow any polynomial where the highest power of x is 2

Example: $x^2 + 3x + 5$

Answer: $x^2 + 3x + 5$

Solution 5:

Polynomial: $x^2 + 1$

Linear polynomial \rightarrow degree 1

Degree of $x^2 + 1 = 2 \rightarrow$ Not linear

Answer: No

Solution 6:

Check whether $x - 2$ is a factor of $x^3 - 3x^2 + 4x - 8$

Use **Remainder Theorem** \rightarrow remainder = $f(2)$

$$f(2) = (2)^3 - 3(2)^2 + 4(2) - 8 = 8 - 12 + 8 - 8 = -4$$

Remainder $\neq 0 \rightarrow x - 2$ is **not a factor**

Answer: Not a factor

Solution 7:

Find remainder when $x^3 + x^2 - x + 2$ is divided by $x + 1$

Remainder = $f(-1)$

$$f(-1) = (-1)^3 + (-1)^2 - (-1) + 2 = -1 + 1 + 1 + 2 = 3$$

Answer: 3

Solution 8:

If α, β are zeroes of $x^2 - 5x + 6 \rightarrow$ sum of zeroes $= \alpha + \beta = -(\text{coefficient of } x)/(\text{coefficient of } x^2)$

$$\alpha + \beta = -(-5)/1 = 5$$

Answer: 5

Solution 9:

Product of zeroes of $2x^2 - 3x + 1 \rightarrow$ product $=$ constant term / coefficient of x^2

$$\alpha\beta = 1 / 2$$

Answer: $\frac{1}{2}$

Solution 10:

Sum of zeroes of $3x^2 + 7x - 6 \rightarrow$ sum $= -(\text{coefficient of } x)/(\text{coefficient of } x^2)$

$$\alpha + \beta = -(7)/3 = -7/3$$

Answer: $-7/3$

Solution 11:

Verify that 1 and -2 are zeroes of $x^2 + x - 2$

$$f(x) = x^2 + x - 2$$

$$f(1) = (1)^2 + 1 - 2 = 0 \quad \checkmark$$

$$f(-2) = (-2)^2 + (-2) - 2 = 4 - 2 - 2 = 0 \quad \checkmark$$

Answer: Both 1 and -2 are zeroes

Solution 12:

Zeroes of $x^2 - 3x + 2 \rightarrow \alpha + \beta = -(-3)/1 = 3, \alpha\beta = 2$

New zeroes = $\alpha + 1, \beta + 1$

Sum of new zeroes = $(\alpha + 1) + (\beta + 1) = \alpha + \beta + 2 = 3 + 2 = 5$

Product of new zeroes = $(\alpha + 1)(\beta + 1) = \alpha\beta + \alpha + \beta + 1 = 2 + 3 + 1 = 6$

Quadratic polynomial = $x^2 - (\text{sum})x + (\text{product}) = x^2 - 5x + 6$

Answer: $x^2 - 5x + 6$

Solution 13:

Sum of zeroes = 5, Product = 6

Quadratic polynomial = $x^2 - (\text{sum})x + (\text{product}) = x^2 - 5x + 6$

Answer: $x^2 - 5x + 6$

Solution 14:

Find zeroes of $2x^2 - 5x - 3$

Use quadratic formula: $x = [5 \pm \sqrt{(25 - 4 \times 2 \times (-3))}]/(2 \times 2) = [5 \pm \sqrt{(25 + 24)}]/4 = [5 \pm \sqrt{49}]/4 = [5 \pm 7]/4$

$x_1 = (5 + 7)/4 = 12/4 = 3$

$x_2 = (5 - 7)/4 = -2/4 = -1/2$

Check sum = $x_1 + x_2 = 3 - 1/2 = 5/2 = -(\text{coefficient of } x)/(\text{coefficient of } x^2) = -(-5)/2 = 5/2$ ✓

Check product = $x_1 \times x_2 = 3 \times (-1/2) = -3/2 = (\text{constant})/(\text{coefficient of } x^2) = -3/2$

Answer: Zeroes are 3 and $-1/2$

Solution 15:

Zeroes of $x^2 - x - 6 \rightarrow \alpha + \beta = 1, \alpha\beta = -6$

Zeroes of new polynomial = $1/\alpha$ and $1/\beta$

Sum = $1/\alpha + 1/\beta = (\alpha + \beta)/\alpha\beta = 1/(-6) = -1/6$ ❌ (check)

Wait step properly: Sum = $(1/\alpha + 1/\beta) = (\alpha + \beta)/(\alpha\beta) = 1/(-6) = -1/6$ ✅

Product = $(1/\alpha)(1/\beta) = 1/(\alpha\beta) = 1/(-6) = -1/6$

Quadratic polynomial = $x^2 - (\text{sum})x + (\text{product}) = x^2 - (-1/6)x + (-1/6) = x^2 + (1/6)x - 1/6$

Multiply by 6 to remove fraction $\rightarrow 6x^2 + x - 1$

Answer: $6x^2 + x - 1$

Question 17

Find a quadratic polynomial whose zeroes are 2 more than the zeroes of

$$x^2 - 3x + 2$$

Solution:

Given polynomial:

$$x^2 - 3x + 2 = 0$$

Let its zeroes be α and β

👉 From standard relations:

$$\alpha + \beta = \frac{3}{1} = 3$$

$$\alpha\beta = \frac{2}{1} = 2$$

New zeroes are:

$$\alpha + 2, \beta + 2$$

Sum of new zeroes:

$$(\alpha + 2) + (\beta + 2) = \alpha + \beta + 4 = 3 + 4 = 7$$

Product of new zeroes:

$$\begin{aligned} &(\alpha + 2)(\beta + 2) \\ &= \alpha\beta + 2(\alpha + \beta) + 4 \\ &= 2 + 2(3) + 4 = 12 \end{aligned}$$

Required quadratic polynomial:

$$\begin{aligned} &x^2 - (\text{sum})x + (\text{product}) \\ &\boxed{x^2 - 7x + 12} \end{aligned}$$

Question 18

Find a cubic polynomial with zeroes 1, -2, 3

Solution:

Zeroes given:

$$1, -2, 3$$

Polynomial:

$$(x - 1)(x + 2)(x - 3)$$

First multiply:

$$(x - 1)(x - 3) = x^2 - 4x + 3$$

Now multiply with $(x + 2)$:

$$\begin{aligned} & (x^2 - 4x + 3)(x + 2) \\ &= x^3 + 2x^2 - 4x^2 - 8x + 3x + 6 \\ &= x^3 - 2x^2 - 5x + 6 \\ & \boxed{x^3 - 2x^2 - 5x + 6} \end{aligned}$$

Question 19

If α and β are zeroes of

$$2x^2 - 5x + 3$$

verify that

$$\frac{1}{\alpha} + \frac{1}{\beta} = \frac{\alpha + \beta}{\alpha\beta}$$

Solution:

Given polynomial:

$$2x^2 - 5x + 3 = 0$$

$$\alpha + \beta = \frac{5}{2}$$

$$\alpha\beta = \frac{3}{2}$$

LHS:

$$\begin{aligned} \frac{1}{\alpha} + \frac{1}{\beta} &= \frac{\alpha + \beta}{\alpha\beta} \\ &= \frac{5/2}{3/2} = \frac{5}{3} \end{aligned}$$

RHS:

$$\frac{\alpha + \beta}{\alpha\beta} = \frac{5/2}{3/2} = \frac{5}{3}$$

LHS = RHS

Hence verified

Question 20

If α, β, γ are zeroes of

$$x^3 - 6x^2 + 11x - 6$$

find $\alpha\beta + \beta\gamma + \gamma\alpha$

Solution:

For cubic polynomial:

$$x^3 + ax^2 + bx + c$$

Sum of products of zeroes two at a time = b

Given:

$$x^3 - 6x^2 + 11x - 6$$

Here,

$$\alpha\beta + \beta\gamma + \gamma\alpha = 11$$

11

Question 21

Check whether $x - 3$ is a factor of

$$x^3 - 4x^2 + x + 6$$

Solution (Remainder Theorem):

Let:

$$P(x) = x^3 - 4x^2 + x + 6$$

Substitute $x = 3$:

$$P(3) = 27 - 36 + 3 + 6 = 0$$

Since remainder = 0,

$$\boxed{x - 3 \text{ is a factor}}$$

Question 22

Find remainder when

$$x^3 + 2x^2 - 5x + 4$$

is divided by $x - 2$

Solution:

By Remainder Theorem:

$$P(2) = 8 + 8 - 10 + 4 = 10$$

$$\boxed{\text{Remainder} = 10}$$

Question 23

Find a quadratic polynomial whose zeroes are squares of zeroes of

$$x^2 - 3x + 2$$

Solution:

Let zeroes be α, β

$$\alpha + \beta = 3$$

$$\alpha\beta = 2$$

New zeroes:

$$\alpha^2, \beta^2$$

Sum:

$$\begin{aligned}\alpha^2 + \beta^2 &= (\alpha + \beta)^2 - 2\alpha\beta \\ &= 9 - 4 = 5\end{aligned}$$

Product:

$$\alpha^2\beta^2 = (\alpha\beta)^2 = 4$$

Polynomial:

$$\begin{array}{c}x^2 - 5x + 4 \\ \boxed{x^2 - 5x + 4}\end{array}$$

Question 24

If α, β are zeroes of

$$x^2 - 2x - 3$$

find polynomial whose zeroes are $\alpha - 1, \beta - 1$

Solution:

$$\alpha + \beta = 2$$

$$\alpha\beta = -3$$

New zeroes:

$$\alpha - 1, \beta - 1$$

Sum:

$$(\alpha + \beta) - 2 = 2 - 2 = 0$$

Product:

$$\begin{aligned}\alpha\beta - (\alpha + \beta) + 1 \\ = -3 - 2 + 1 = -4\end{aligned}$$

Polynomial:

$$\begin{aligned}x^2 - 4 \\ \boxed{x^2 - 4}\end{aligned}$$

Solution 25

Let the zeroes of the given polynomial be α and β .

Given polynomial:

$$\begin{aligned}x^2 - 5x + 6 \\ \alpha + \beta = 5, \alpha\beta = 6\end{aligned}$$

We know,

$$\begin{aligned}\alpha^3 + \beta^3 &= (\alpha + \beta)^3 - 3\alpha\beta(\alpha + \beta) \\ &= 5^3 - 3(6)(5) \\ &= 125 - 90 \\ &= \boxed{35}\end{aligned}$$

Solution 26

Let the zeroes of the given polynomial be α and β .

Given polynomial:

$$\begin{aligned}x^2 - x - 6 \\ \alpha + \beta = 1, \alpha\beta = -6\end{aligned}$$

Required zeroes:

$$\frac{1}{\alpha}, \frac{1}{\beta}$$

Sum of new zeroes:

$$\frac{1}{\alpha} + \frac{1}{\beta} = \frac{\alpha + \beta}{\alpha\beta} = \frac{1}{-6} = -\frac{1}{6}$$

Product of new zeroes:

$$\frac{1}{\alpha\beta} = -\frac{1}{6}$$

Required quadratic polynomial:

$$x^2 - (\text{sum})x + (\text{product})$$
$$x^2 + \frac{1}{6}x - \frac{1}{6}$$

Multiplying throughout by 6:

$$\boxed{6x^2 + x - 1}$$

Solution 27

Given cubic polynomial:

$$x^3 - 3x^2 + 4x - 2$$

Let zeroes be α, β, γ .

$$\alpha + \beta + \gamma = 3$$
$$\alpha\beta + \beta\gamma + \gamma\alpha = 4$$

We know,

$$\begin{aligned}\alpha^2 + \beta^2 + \gamma^2 &= (\alpha + \beta + \gamma)^2 - 2(\alpha\beta + \beta\gamma + \gamma\alpha) \\ &= 3^2 - 2(4) \\ &= 9 - 8 \\ &= \boxed{1}\end{aligned}$$

Solution 28

Let the zeroes of the given polynomial be α and β .

Given polynomial:

$$\begin{aligned}x^2 - 7x + 12 \\ \alpha + \beta = 7\end{aligned}$$

LHS:

$$\begin{aligned}\alpha^2 - \beta^2 &= (\alpha - \beta)(\alpha + \beta) \\ &= (\alpha - \beta)(7)\end{aligned}$$

RHS:

$$\begin{aligned}(\alpha - \beta)(\alpha + \beta) &= (\alpha - \beta)(7) \\ \text{LHS} &= \text{RHS}\end{aligned}$$

Hence verified

Solution 29

Given zeroes:

$$1, -1, 2$$

Required cubic polynomial:

$$(x-1)(x+1)(x-2)$$

$$= (x^2 - 1)(x - 2)$$

$$= x^3 - 2x^2 - x + 2$$
$$\boxed{x^3 - 2x^2 - x + 2}$$

Solution 30

Given polynomial:

$$P(x) = 2x^3 + 3x^2 - x + 5$$

By Remainder Theorem:

$$\begin{aligned}\text{Remainder} &= P(-1) \\ &= 2(-1)^3 + 3(-1)^2 - (-1) + 5 \\ &= -2 + 3 + 1 + 5 \\ &= \boxed{7}\end{aligned}$$